\documentclass[10pt]{article}
\usepackage{amsmath}
\usepackage{mathrsfs}
\usepackage{amssymb}
\usepackage{graphicx}
\usepackage{caption}
\usepackage{subcaption}
\usepackage[margin=1in]{geometry}

\begin{document}
\begin{equation}
F^\sigma_{\mu\nu} = h_{\mu\nu} + G^\sigma_{\mu\nu}
\end{equation}
\begin{align}
G^\sigma_{\mu\nu} &= \sum_{\lambda\kappa}(\mu\nu\vert\lambda\kappa)P^T_{\kappa\lambda} -\sum_{\lambda\kappa}(\mu\kappa\vert\lambda\nu)P^\sigma_{\kappa\lambda}\\
&=\sum_{\lambda\kappa}(\mu\nu\vert\lambda\kappa)P^T_{\kappa\lambda} -\frac{1}{2}\sum_{\lambda\kappa}(\mu\kappa\vert\lambda\nu)P^\sigma_{\kappa\lambda} -\frac{1}{2}\sum_{\lambda\kappa}(\mu\kappa\vert\lambda\nu)P^\sigma_{\kappa\lambda}\\
&=\sum_{\lambda\kappa}(\mu\nu\vert\lambda\kappa)P^T_{\kappa\lambda} -\frac{1}{2}\sum_{\lambda\kappa}(\mu\kappa\vert\lambda\nu)P^\sigma_{\kappa\lambda} -\frac{1}{2}\sum_{\lambda\kappa}(\mu\lambda\vert\kappa\nu)P^\sigma_{\lambda\kappa}\\
&=\sum_{\lambda\kappa}(\mu\nu\vert\lambda\kappa)P^T_{\kappa\lambda} -\frac{1}{2}\sum_{\lambda\kappa}(\mu\kappa\vert\nu\lambda)P^\sigma_{\kappa\lambda} -\frac{1}{2}\sum_{\lambda\kappa}(\mu\lambda\vert\nu\kappa)P^{\sigma}_{\lambda\kappa} \qquad\qquad (\mu\nu\vert\lambda\kappa)\in\mathbb{R}\\
&=\sum_{\lambda\kappa}(\mu\nu\vert\lambda\kappa)P^T_{\kappa\lambda} -\frac{1}{2}\sum_{\lambda\kappa}(\mu\kappa\vert\nu\lambda)P^\sigma_{\kappa\lambda} -\frac{1}{2}\sum_{\lambda\kappa}(\mu\lambda\vert\nu\kappa)P^{\sigma*}_{\kappa\lambda} \qquad\qquad \mathbf{P}=\mathbf{P}^\dagger
\end{align}
\begin{align}
&G^\sigma_{\mu\nu} = G^\sigma_{\mu\nu} + (\mu\nu\vert\lambda\kappa)P^T_{\kappa\lambda}\\
&G^\sigma_{\lambda\kappa} = G^\sigma_{\lambda\kappa} + (\mu\nu\vert\lambda\kappa)P^T_{\nu\mu}\\
\end{align}
\end{document}